examples/conn/proofs.v
@@ -28,6 +28,12 @@ Implicit Types γ : gname.
 Implicit Types v : val.
 Implicit Types (N : namespace).
 
+Lemma wp_channel cs :
+  {{{ True }}}
+    impl.channel (repr cs)
+  {{{ RET (GenConn.cs_chan cs); True }}}.
+Proof. exact: GenConn.wp_channel. Qed.
+
 Lemma wp_connect P c skI skR N ps :
   channel c ∗
   cryptis_ctx ∗
@@ -44,8 +50,8 @@ Lemma wp_connect P c skI skR N ps :
 Proof. exact: GenConn.wp_connect. Qed.
 
 Lemma wp_listen c N ps :
-  channel c -∗
-  cryptis_ctx -∗
+  channel c ∗
+  cryptis_ctx ∗
   ctx N ps -∗
   {{{ True }}}
     impl.listen c
@@ -56,9 +62,11 @@ Proof. exact: GenConn.wp_listen. Qed.
 Lemma wp_confirm P ps c skI skR ga N :
   channel c ∗
   cryptis_ctx ∗
-  ctx N ps -∗
-  {{{ public ga ∗ minted skI ∗ minted skR ∗
-      (GenConn.failure skI skR ∨ P) }}}
+  ctx N ps ∗
+  public ga ∗
+  minted skI ∗
+  minted skR -∗
+  {{{ GenConn.failure skI skR ∨ P }}}
     impl.confirm c skR (Tag N) (ga, Spec.pkey skI)%V
   {{{ cs, RET (repr cs);
       connected ps skI skR Resp cs ∗
@@ -66,24 +74,26 @@ Lemma wp_confirm P ps c skI skR ga N :
       release_token (si_resp_share cs) ∗
       term_token (si_resp_share cs) (⊤ ∖ ↑iso_dhN ∖ ↑connN) }}}.
 Proof.
-iIntros "#? !> %Φ (#p_ga & #p_pkA & #sign_skB & P) post".
-wp_apply (GenConn.wp_confirm P with "[//] [$P]") => //.
-do !iSplit => //=. by eauto.
+iIntros "(#? & #ctx & #? & #p_ga & #p_pkA & #sign_skB)".
+iApply GenConn.wp_confirm.
+iFrame "#". iIntros "!> % _ !>".
+by rewrite /base.chan_inv /=; eauto.
 Qed.
 
 Lemma wp_send skI skR rl cs t N ps :
-  ctx N ps -∗
+  ctx N ps ∗
   public t -∗
   {{{ connected ps skI skR rl cs ∗
       (public (si_key cs) ∨ msg_inv ps skI skR cs rl t) }}}
     impl.send (repr cs) t
   {{{ RET #(); connected ps skI skR rl cs }}}.
 Proof.
-iIntros "#ctx #p_t !> %Φ (conn & inv) post".
+iIntros "#ctx !> %Φ (conn & inv_t) post".
 wp_apply (GenConn.wp_send (λ skI skR si, True)%I
-  with "[//] [//] [$conn inv]") => //.
-- iDestruct "inv" as "[fail|inv]"; auto.
-  iRight. iIntros "% % [inv1 inv2]".
+  with "[] [$conn inv_t]").
+- by iFrame "#".
+- iDestruct "inv_t" as "[fail|inv_t]"; first by eauto.
+- iRight. iIntros "% % [inv1 inv2]".
   by case: rl; iFrame; eauto.
 - iIntros "[? _]". by iApply "post".
 Qed.
